Added LogicalRelations.v, which defined the two distinct notions of distinguished equalities and logical relations between types with distinguished equalities; updated the Monad typeclass with this change, and started updated PredMonad...

Monad.v
@@ -1,56 +1,6 @@
 
-Require Import Coq.Program.Tactics.
-Require Import Coq.Setoids.Setoid.
-Require Import Coq.Classes.Morphisms.
-Require Import Coq.Arith.Arith_base.
-Require Import Coq.Relations.Relations.
-
-
-(***
- *** Logical Relations
- ***)
-
-(* A logical relation is just an equivalence with a fancy name, so that we can
-distinguish them as "the" relations for their respective types *)
-Polymorphic Class LogRel_Rel@{c} (A : Type@{c}) : Type :=
-  equalsLR : A -> A -> Prop.
-
-(* The propositional part of a logical relation *)
-Polymorphic Class LogRel@{c} (A : Type@{c}) {LR:LogRel_Rel A} : Prop :=
-  { logrel_equivalence :> Equivalence equalsLR }.
-
-Notation "x '==' y" := (equalsLR x y) (at level 80, no associativity).
-
-(* equalsLR respects itself *)
-(* FIXME: this is probably not needed...? *)
-(*
-Polymorphic Instance equalsLR_proper `{LogRel} :
-  Proper (equalsLR ==> equalsLR ==> iff) equalsLR.
-intros x1 x2 ex y1 y2 ey. rewrite ex.
- split; intro exy.
-rewrite <- ex; rewrite exy; rewrite ey; reflexivity.
-rewrite ex; rewrite exy; rewrite <- ey; reflexivity.
-Qed.
-*)
-
-
-(* Some standard logical relations *)
-
-Polymorphic Instance Pair_LogRel_Rel (A B: Type)
-            {LRA:LogRel_Rel A} {LRB:LogRel_Rel B} : LogRel_Rel (A*B) :=
-  fun p1 p2 =>
-    equalsLR (fst p1) (fst p2) /\ equalsLR (snd p1) (snd p2).
-
-Polymorphic Instance Pair_LogRel (A B: Type)
-            `{LRA:LogRel A} `{LRB:LogRel B} : LogRel (A*B).
-  repeat constructor.
-  reflexivity.
-  reflexivity.
-  destruct H; symmetry; assumption.
-  destruct H; symmetry; assumption.
-  destruct H; destruct H0; transitivity (fst y); assumption.
-  destruct H; destruct H0; transitivity (snd y); assumption.
-Qed.
+Add LoadPath "." as PredMonad.
+Require Export PredMonad.LogicalRelations.
 
 
 (***
@@ -60,29 +10,29 @@ Qed.
 Polymorphic Class MonadOps@{d c} (M : Type@{d} -> Type@{c}) : Type :=
   { returnM : forall {A : Type@{d}}, A -> M A;
     bindM : forall {A B : Type@{d}}, M A -> (A -> M B) -> M B;
-    equalsM :> forall {A : Type@{d}} {LR:LogRel_Rel A}, LogRel_Rel (M A) }.
+    equalsM :> forall {A : Type@{d}} `{EqualsOp A}, EqualsOp (M A) }.
 
 Polymorphic Class Monad@{d c} (M : Type@{d} -> Type@{c})
             {MonadOps:MonadOps@{d c} M} : Prop :=
   {
     monad_return_bind :
-      forall (A B:Type@{d}) `{LogRel B} x (f:A -> M B),
+      forall (A B:Type@{d}) `{Equals B} x (f:A -> M B),
         bindM (returnM x) f == f x;
     monad_bind_return :
-      forall (A:Type@{d}) (m:M A) `{LogRel A},
+      forall (A:Type@{d}) (m:M A) `{Equals A},
         bindM m returnM == m;
     monad_assoc :
-      forall (A B C:Type@{d}) `{LogRel C} m (f:A -> M B) (g:B -> M C),
+      forall (A B C:Type@{d}) `{Equals C} m (f:A -> M B) (g:B -> M C),
         bindM (bindM m f) g == bindM m (fun x => bindM (f x) g);
     monad_equalsM :>
-      forall (A:Type@{d}) `{LogRel A},
-        LogRel _ (LR:=equalsM);
+      forall (A:Type@{d}) `{Equals A},
+        Equals _ (Eq:=equalsM);
     monad_proper_return :>
-      forall (A:Type@{d}) `{LogRel A},
-        Proper (equalsLR ==> equalsM) returnM;
+      forall (A:Type@{d}) `{Equals A},
+        Proper (equals ==> equalsM) returnM;
     monad_proper_bind :>
-      forall (A B:Type@{d}) `{LogRel A} `{LogRel B},
-        Proper (equalsM ==> (equalsLR ==> equalsM) ==> equalsM)
+      forall (A B:Type@{d}) `{Equals A} `{Equals B},
+        Proper (equalsM ==> (equals ==> equalsM) ==> equalsM)
                (bindM (A:=A) (B:=B))
   }.
 
@@ -92,42 +42,42 @@ Polymorphic Class Monad@{d c} (M : Type@{d} -> Type@{c})
  ***)
 
 (* FIXME: Equivalence and friends are not polymorphic... *)
-Instance equalsM_Equivalence `{Monad} `{LogRel} : Equivalence (equalsM (A:=A)).
+Instance equalsM_Equivalence `{Monad} `{Equals} : Equivalence (equalsM (A:=A)).
   apply monad_equalsM; assumption.
 Qed.
 
 (* FIXME: why is this not automatic in the proof of bind_fun_equalsM?!? *)
-Instance equalsM_Reflexive `{Monad} `{LogRel} : Reflexive (equalsM (A:=A)).
+Instance equalsM_Reflexive `{Monad} `{Equals} : Reflexive (equalsM (A:=A)).
   auto with typeclass_instances.
 Qed.
 
-Instance equalsM_Symmetric `{Monad} `{LogRel} : Symmetric (equalsM (A:=A)).
+Instance equalsM_Symmetric `{Monad} `{Equals} : Symmetric (equalsM (A:=A)).
   auto with typeclass_instances.
 Qed.
 
-Instance equalsM_Transitive `{Monad} `{LogRel} : Transitive (equalsM (A:=A)).
+Instance equalsM_Transitive `{Monad} `{Equals} : Transitive (equalsM (A:=A)).
   auto with typeclass_instances.
 Qed.
 
-Polymorphic Instance equalsM_equalsLR_iff_Proper `{Monad} `{LogRel} :
-  Proper (equalsLR ==> equalsLR ==> iff) equalsM.
+Polymorphic Instance equalsM_equals_iff_Proper `{Monad} `{Equals} :
+  Proper (equals ==> equals ==> iff) equalsM.
 intros m11 m12 e1 m21 m22 e2; split; intros.
 transitivity m11; [ symmetry; assumption | transitivity m21; assumption ].
 transitivity m12; [ assumption |
                     transitivity m22; try assumption; symmetry; assumption ].
 Qed.
 
-Polymorphic Instance equalsM_equalsLR_impl_Proper `{Monad} `{LogRel} :
-  Proper (equalsLR ==> equalsLR ==> Basics.flip Basics.impl) equalsM.
+Polymorphic Instance equalsM_equals_impl_Proper `{Monad} `{Equals} :
+  Proper (equals ==> equals ==> Basics.flip Basics.impl) equalsM.
 intros m11 m12 e1 m21 m22 e2 e12.
 transitivity m12; [ assumption |
                     transitivity m22; try assumption; symmetry; assumption ].
 Qed.
 
 Lemma bind_fun_equalsM `{Monad}
-            {A B:Type} `{LogRel (A:=A)} `{LogRel (A:=B)}
+            {A B:Type} `{Equals (A:=A)} `{Equals (A:=B)}
             m (f1 f2:A -> M B) :
-  Proper (equalsLR ==> equalsM) f1 -> Proper (equalsLR ==> equalsM) f2 ->
+  Proper (equals ==> equalsM) f1 -> Proper (equals ==> equalsM) f2 ->
   (forall x, f1 x == f2 x) -> bindM m f1 == bindM m f2.
 intros proper1 proper2 e; apply (monad_proper_bind A B); [ reflexivity | ].
 intros x y e'.
