LogicalRelations.v
@@ -1,0 +1,108 @@
+
+Require Export Coq.Program.Tactics.
+Require Export Coq.Setoids.Setoid.
+Require Export Coq.Classes.Morphisms.
+Require Export Coq.Arith.Arith_base.
+Require Export Coq.Relations.Relations.
+
+(***
+ *** Distinguished Equalities
+ ***)
+
+(* A distinguished equality is an equality relation marked as "the" equality
+relation for a given type *)
+Polymorphic Class EqualsOp@{c} (A : Type@{c}) : Type :=
+  equals : A -> A -> Prop.
+
+(* Distinguished equalities must be equivalences *)
+Polymorphic Class Equals@{c} (A : Type@{c}) `{Eq:EqualsOp@{c} A} : Prop :=
+  { equals_equivalence :> Equivalence equals }.
+
+Notation "x '==' y" := (equals x y) (at level 80, no associativity).
+
+
+(***
+ *** Equality Instances
+ ***)
+
+(* Equality on pairs = equality on the two components *)
+Polymorphic Instance Pair_EqualsOp (A B: Type)
+            `{EqualsOp A} `{EqualsOp B} : EqualsOp (A*B) :=
+  fun p1 p2 => equals (fst p1) (fst p2) /\ equals (snd p1) (snd p2).
+
+(* Pair equality is a valid equality *)
+Polymorphic Instance Pair_Equals (A B: Type)
+            `{Equals A} `{Equals B} : Equals (A*B).
+  repeat constructor.
+  reflexivity.
+  reflexivity.
+  destruct H1; symmetry; assumption.
+  destruct H1; symmetry; assumption.
+  destruct H1; destruct H2; transitivity (fst y); assumption.
+  destruct H1; destruct H2; transitivity (snd y); assumption.
+Qed.
+
+
+(***
+ *** Logical Relations
+ ***)
+
+(* A logical relation is a relation between two types that respects the
+distinguished equalities of those two types; i.e., it is a morphism in the
+category of equality relations. *)
+Polymorphic Class LogRelOp@{c} (A B : Type@{c}) : Type :=
+  relLR : A -> B -> Prop.
+
+(* The propositional part of a logical relation *)
+Polymorphic Class LogRel@{c} (A B : Type@{c})
+            `{EqA:Equals A} `{EqB:Equals B} `{LR:LogRelOp A B} : Prop :=
+  { logrel_proper :> Proper (equals ==> equals ==> iff) (relLR (A:=A) (B:=B)) }.
+
+Notation "x '~~' y" := (relLR x y) (at level 80, no associativity).
+
+
+(* equals respects itself *)
+(* FIXME: this is probably not needed...? *)
+(*
+Polymorphic Instance equals_proper `{LogRel} :
+  Proper (equals ==> equals ==> iff) equals.
+intros x1 x2 ex y1 y2 ey. rewrite ex.
+ split; intro exy.
+rewrite <- ex; rewrite exy; rewrite ey; reflexivity.
+rewrite ex; rewrite exy; rewrite <- ey; reflexivity.
+Qed.
+*)
+
+
+(***
+ *** Logical Relations
+ ***)
+
+(* The identity logical relation, between a type and itself, is just the type's
+distinguished equality *)
+Polymorphic Instance LogRelOp_Id (A: Type) `{EqualsOp A} : LogRelOp A A :=
+  equals.
+
+Polymorphic Instance LogRel_Id (A: Type) `{Equals A} : LogRel A A.
+constructor; intros x1 x2 ex y1 y2 ey.
+rewrite ex; rewrite ey; reflexivity.
+Qed.
+
+(* The logical relation for pairs: relate the components pointwise *)
+Polymorphic Instance LogRelOp_Pair (A1 A2 B1 B2: Type)
+            `{LogRelOp A1 B1} `{LogRelOp A2 B2} : LogRelOp (A1*A2) (B1*B2) :=
+  fun p1 p2 => fst p1 ~~ fst p2 /\ snd p1 ~~ snd p2.
+
+Polymorphic Instance LogRel_Pair (A1 A2 B1 B2: Type)
+            `{LogRel A1 B1} `{LogRel A2 B2} : LogRel (A1*A2) (B1*B2).
+constructor; intros p1 p1' e1 p2 p2' e2.
+destruct e1 as [e1_1 e1_2]; destruct e2 as [e2_1 e2_2].
+destruct p1; destruct p1'; destruct p2; destruct p2'.
+split; intro e; destruct e as [e_1 e_2]; split;
+unfold fst in * |- *; unfold snd in * |- *.
+rewrite <- e1_1; rewrite <- e2_1; assumption.
+rewrite <- e1_2; rewrite <- e2_2; assumption.
+rewrite e1_1; rewrite e2_1; assumption.
+rewrite e1_2; rewrite e2_2; assumption.
+Qed.
+
